## **Reverse a String Recursively**

### **Problem**

Given a string `s`, return a new string which is the **reverse** of `s` using recursion.

**Example:**

* Input: `"hello"`
* Output: `"olleh"`

---

### **Key Concepts**

1. **Base Case** – When the recursion should stop.

   * If the string is empty (`""`) or has **one character**, it is already reversed.
2. **Recursive Case** – Break the problem into smaller sub-problems.

   * Reverse the substring **excluding the first character**, then append the first character to the **end** of the reversed substring.

---

### **Mathematical / Conceptual Idea**

Let `reverse(s)` reverse string `s`.

[
\text{reverse}("hello") = \text{reverse}("ello") + "h"
]

[
\text{reverse}("ello") = \text{reverse}("llo") + "e"
]

…and so on, until we reach the base case.

---

### **Step-by-Step Example: `"cat"`**

1. `reverse("cat")` → `reverse("at") + "c"`
2. `reverse("at")` → `reverse("t") + "a"`
3. `reverse("t")` → `"t"` (base case reached)

Now the recursion **unwinds**:

```
reverse("t") = "t"
reverse("at") = "t" + "a" = "ta"
reverse("cat") = "ta" + "c" = "tac"
```

---

### **Code Example (Java)**

```java
public class ReverseString {
    public static String reverse(String str) {
        // Base case: empty string or single character
        if (str == null || str.length() <= 1) {
            return str;
        }
        // Recursive case
        return reverse(str.substring(1)) + str.charAt(0);
    }

    public static void main(String[] args) {
        String s = "cat";
        System.out.println("Reversed: " + reverse(s)); // Output: "tac"
    }
}
```

---

### **Key Points**

1. Base case ensures **termination** of recursion.
2. Recursive case reduces the problem size by **removing the first character**.
3. Each recursive call is stored on the **call stack**, then the string is rebuilt in reverse order during **stack unwind**.
4. Time Complexity: O(n)
5. Space Complexity: O(n) due to recursion stack

---

### **Visualizing Call Stack for `"cat"`**

```
reverse("cat") → reverse("at") + "c"
reverse("at") → reverse("t") + "a"
reverse("t") → "t"
Stack unwinds:
reverse("at") = "t" + "a" = "ta"
reverse("cat") = "ta" + "c" = "tac"
```
